Adding context and predicates

src/Basics.lean
@@ -1,21 +1,50 @@
-
-
+-- We start by defining our basic type base and the arrow type --
 inductive Typ : Type
   | base : Typ
   | arrow : Typ → Typ → Typ
 
+-- Print function for convenience --
+def printTyp (t : Typ) : String := by 
+  cases t 
+  case base => exact " base " 
+  case arrow t₁ t₂ => exact printTyp t₁ ++ "→" ++ printTyp t₂ 
+
 namespace Typ
 
-
+-- We define a context, which is just a list of variable and types --
 inductive Ctx : Type
   | nil   : Ctx
-  | cons  : Nat → Typ → Ctx → Ctx 
+  | cons  (n : Nat)  (t : Typ) (c : Ctx ) : Ctx 
+
+-- A type that is inhabited whenever a variable is not present in a context --
+inductive notInCtx (n : Nat) (t : Typ) : Ctx → Type 
+  | nil : notInCtx n t Ctx.nil
+  | cons (n₁ : Nat) (t₁ : Typ) (p₁ : Ctx) (p : n ≠ n₁) : notInCtx n t (Ctx.cons n₁ t₁ p₁)
+
+-- A type that is inhabited whenever a context is valid, i.e does not contain duplicates --
+inductive validCtx : Ctx → Type
+  | nil : validCtx nil
+  | cons (n : Nat) (t : Typ) (c : Ctx) (p : notInCtx n t c) : validCtx (Ctx.cons n t c)
 
 namespace Ctx
+def printCtx (c : Ctx) : String := by
+  cases c
+  case nil => exact ""
+  case cons n t c  => exact "(" ++ toString n ++ printTyp t ++ ")" ++ printCtx c
 
-def ctx₁ : Ctx := cons 2 base nil
+-- Let's define a context and prove that it is a valid one --
+-- Note that if we define an invalid context, there will be no proof of it being valid --
+def ctx₁ : Ctx := cons 2 base (cons 3 (arrow base base) nil)
 #check ctx₁ 
-#eval ctx₁ 
+#eval printCtx ctx₁ 
+
+-- A Proof that the previous context is a valid context --
+example : validCtx ctx₁ := by
+  apply validCtx.cons 
+  apply notInCtx.cons 
+  trivial
+
+
 
 
 end Ctx
